coq/BaseExpressions/PrimOps.v
@@ -1,0 +1,25 @@
+From Cofq.BaseExpressions Require Import Integers.
+
+Inductive PrimOp : Set :=
+| Mul
+| Add
+| Sub
+.
+
+Definition eval_primop {I} `{FInt I} (op : PrimOp) : (I -> I -> I) :=
+  match op with
+  | Mul => mul
+  | Add => add
+  | Sub => sub
+  end.
+
+Definition eval_op {I} `{FInt I} (op : PrimOp) (x y : I) : I :=
+  eval_primop op x y.
+
+Definition op_eq (op1 op2 : PrimOp) : bool
+  := match op1, op2 with
+     | Mul, Mul => true
+     | Add, Add => true
+     | Sub, Sub => true
+     | _, _ => false
+     end.
