coq/Show/ShowUtils.v
@@ -1,0 +1,50 @@
+From Coq Require Import ZArith String List.
+From QuickChick Require Export Show.
+
+Global Open Scope string_scope.
+
+From Cofq.BaseExpressions Require Import PrimOps.
+
+Variant Precedence :=
+| PrecOuter
+| PrecMult
+| PrecAdd
+| PrecSub
+| PrecApp
+| PrecInner
+.
+
+Definition prec_value (p : Precedence) : N :=
+  match p with
+  | PrecOuter => 0
+  | PrecAdd => 1
+  | PrecSub => 1
+  | PrecMult => 2
+  | PrecApp => 3
+  | PrecInner => 4
+  end.
+
+Definition parens (outer inner : Precedence) (s : string) :=
+  if N.leb (prec_value outer) (prec_value inner)
+  then s
+  else "(" ++ s ++ ")".
+
+Definition intersperse (sep : string) (l : list string) : string
+  := fold_left (fun acc s => if eqb "" acc then s else s ++ sep ++ acc) l "".
+
+Instance showPrimOp : Show PrimOp :=
+  {| show :=
+       fun (op : PrimOp) =>
+         match op with
+         | Mul => "*"
+         | Add => "+"
+         | Sub => "-"
+         end
+  |}.
+
+Definition op_prec (op : PrimOp) : Precedence
+  := match op with
+     | Mul => PrecMult
+     | Add => PrecAdd
+     | Sub => PrecSub
+     end.
