coq/SystemF/SystemFDefinitions.v
@@ -1,0 +1,79 @@
+From Coq Require Export
+     ZArith
+     String
+     List.
+
+From Vellvm Require Import
+     Numeric.Integers
+     Utils.Util.
+
+From ITree Require Import
+     Basics
+     ITree
+     Interp.Recursion
+     Events.Exception.
+
+From QuickChick Require Import Show.
+
+From Cofq.BaseExpressions Require Export
+     Integers
+     PrimOps.
+
+From Cofq.Utils Require Import
+     Utils.
+
+Notation TypeInd := N.
+Notation VarInd  := N.
+
+Unset Elimination Schemes.
+Inductive FType : Set :=
+| Arrow   : FType -> FType -> FType
+| Prod    : list FType -> FType
+| TForall : FType -> FType
+| TVar    : TypeInd -> FType
+(* Base Types *)
+| IntType   : FType
+.
+Set Elimination Schemes.
+
+Section FTypeInd.
+  Variable P : FType -> Prop.
+  Hypothesis IH_IntType       : P IntType.
+  Hypothesis IH_TVar          : forall x, P (TVar x).
+  Hypothesis IH_Prod          : forall (ts: list FType), (forall t, In t ts -> P t) -> P (Prod ts).
+  Hypothesis IH_Arrow         : forall t1 t2, P t1 -> P t2 -> P (Arrow t1 t2).
+  Hypothesis IH_TForall       : forall t, P t -> P (TForall t).
+
+  Lemma FType_ind : forall (t:FType), P t.
+    fix IH 1.
+    remember P as P0 in IH.
+    destruct t; auto; subst.
+    - apply IH_Arrow; auto.
+    - apply IH_Prod.
+      { revert l.
+        fix IH_ts 1. intros [|u ts']. intros. inversion H.
+        intros u' [<-|Hin]. apply IH. eapply IH_ts. apply Hin.
+      }
+    - apply IH_TForall. auto.
+  Qed.
+End FTypeInd.
+
+Inductive Term {I} `{FInt I} : Type :=
+| Var          : VarInd -> Term
+(* Annotated terms *)
+| Ann          : Term -> FType -> Term
+(* Terms *)
+| Fix          : FType -> FType -> Term -> Term
+| App          : Term -> Term -> Term
+(* Type stuff *)
+| TAbs         : Term -> Term
+| TApp         : Term -> FType -> Term
+(* Prod *)
+| Tuple        : list Term -> Term 
+| ProjN        : N -> Term -> Term
+(* Int *)
+| Num          : I -> Term
+(* Expressions *)
+| If0          : Term -> Term -> Term -> Term
+| Op           : PrimOp -> Term -> Term -> Term
+.
