coq/Test/TestUtils.v
@@ -1,0 +1,27 @@
+From Coq Require Import
+     String.
+
+From QuickChick Require Import Show.
+Set Warnings "-extraction-opaque-accessed,-extraction".
+
+(* I don't know why, but I need this to make Extract Inductive work below... *)
+From ITree Require Import
+     ITree.
+
+Global Open Scope string_scope.
+
+Inductive MlResult a e :=
+| MlOk : a -> MlResult a e
+| MlError : e -> MlResult a e
+.
+
+Extract Inductive MlResult => "result" [ "Ok" "Error" ].
+
+Instance showMLResult {A E} `{Show A} `{Show E} : Show (MlResult A E)
+  := {| show :=
+          fun mlr =>
+            match mlr with
+            | @MlOk _ _ x => "MlOk " ++ show x
+            | @MlError _ _ x => "MlError " ++ show x
+            end
+    |}.
