coq/Utils/Utils.v
@@ -1,0 +1,41 @@
+From Coq Require Import List Lia.
+
+Global Open Scope list_scope.
+
+(* Check that a predicate holds elementwise across two lists, while
+   also making sure that the lists have equal length.
+*)
+Fixpoint zip_pred {X Y} (pred : X -> Y -> bool) (xs : list X) (ys : list Y) : bool
+  := match xs, ys with
+     | nil, nil => true
+     | x::xs, y::ys => pred x y && zip_pred pred xs ys
+     | _, _ => false
+     end.
+
+Lemma list_sum_map :
+  forall {X} (f : X -> nat) x xs,
+    In x xs ->
+    list_sum (map f xs) >= f x.
+Proof.
+  induction xs; intros In; [contradiction|].
+  destruct In; subst.
+  - cbn. lia.
+  - cbn. specialize (IHxs H).
+    unfold list_sum in IHxs.
+    lia.
+Qed.
+
+Lemma map_In {A B : Type} (l : list A) (f : forall (x : A), In x l -> B) : list B.
+Proof.
+  induction l.
+  - exact nil.
+  - refine (f a _ :: IHl _).
+    + simpl. auto.
+    + intros x H. apply (f x). simpl. auto.
+Defined.
+
+Fixpoint zipwith {X Y Z} (f : X -> Y -> Z) (xs : list X) (ys : list Y) : list Z
+  := match xs, ys with
+     | (x :: xs), (y :: ys) => f x y :: (zipwith f xs ys)
+     | _, _ => nil
+     end.
